@prefix mv: <http://eccenca.com/mobivoc/> .
@prefix owl: <http://www.w3.org/2002/07/owl#> .
@prefix rdf: <http://www.w3.org/1999/02/22-rdf-syntax-ns#> .
@prefix rdfs: <http://www.w3.org/2000/01/rdf-schema#> .
@prefix skos: <http://www.w3.org/2004/02/skos/core#> .
@prefix geo: <http://www.w3.org/2003/01/geo/wgs84_pos#> .
@prefix vcard: <http://www.w3.org/2006/vcard/ns#> .


mv:FillingStation
	a rdfs:Class , owl:Class ;
	rdfs:comment "Facility for combustion motor vehicles or electric motor vehicle." ;
	rdfs:label "filling station"@en, "Abfullstation"@de .
	
mv:FuelStation
	rdfs:subClassOf mv:FillingStation ;
	rdfs:comment "Facility for refueling motor vehicle." ;
	rdfs:label "fuel station"@en, "Tankstelle"@de ;
	skos:altLabel "petrol station"@en , "gas station"@en-US. # property is used when synonyms, near-synonyms, or abbrevia- tions need to be represented.

mv:ChargingStation
	rdfs:subClassOf mv:FillingStation ; 
	rdfs:comment "Facility for electric motor vehicle." ;
	rdfs:label "charging station"@en, "Ladestation"@de .


# Properties

mv:ChargingStationName
	a rdf:Property , owl:DatatypeProperty ;
	rdfs:comment "Indicates the name of the charging station" ;
	rdfs:label "charging station name"@en , "Ladestationnnummer"@de ;
	rdfs:domain mv:ChargingStation ;
	rdfs:range rdfs:Literal .
	
mv:fillingStationNumber
	a rdf:Property , owl:DatatypeProperty ;
	rdfs:comment "Indicates the unique number of the filling station." ;
	rdfs:label "filling station number"@en , "Tankstellennummer"@de ;
	rdfs:domain mv:FillingStation ;
	rdfs:range rdfs:Literal .

mv:fillingStationHeight
	a rdf:Property , owl:DatatypeProperty ;
	rdfs:comment "Indicates the height of the filling station. This is important especially for trucks" ;
	rdfs:label "filling station height"@en, "Tankstelle heit"@de ;
	rdfs:domain mv:FuelStation ;
	rdfs:range rdfs:Literal .
	
mv:hasIdentifications
	a rdf:Property , owl:ObjectProperty ;
	rdfs:comment "Way of identifying the booked vehicle" ;
	rdfs:label "has identifications"@en, "hat Identifikation"@de;
	rdfs:domain mv:ChargingStation ;
	rdfs:range mv:Fuel .

mv:hasOffer
	a rdf:Property , owl:ObjectProperty ;
	rdfs:comment "Indicates the sort of fuels product the filling station offers." ;
	rdfs:label "has offer"@en, "hat Angebot"@de ;
	rdfs:domain mv:FuelStation ;
	rdfs:range mv:Fuel .

mv:hasParkingFacility
	a rdf:Property, owl:DatatypeProperty ;
	rdfs:comment "Indicates what kind of parking facilities the station has" ;
	rdfs:label "has parking facility"@en, "hat Parkmoglichkeit"@de ;
	rdfs:domain mv:FuelStation ;
	rdfs:range rdfs:Literal .

mv:hasPrice
	a rdf:Property, owl:DatatypeProperty ;
	rdfs:comment "Indicates the information about the price of the facilities." ;
	rdfs:label "has price"@en, "hat Preis"@de ;
	rdfs:domain mv:FuelStation;
	rdfs:range rdfs:Literal .

mv:hasShoppingFacility
	a rdf:Property, owl:DatatypeProperty ;
	rdfs:comment "Indicate whether Filling Station has Shopping Facility or not" ;
	rdfs:label "has shopping facility"@en, "weist Einkaufsgelenheit"@de ;
	rdfs:domain mv:FuelStation ;
	rdfs:range rdfs:Literal .

mv:hasWashingFacility
	a rdf:Property, owl:DatatypeProperty ;
	rdfs:comment "Indicate whether Filling Station has Washing Facility or not" ;
	rdfs:label "has washing facility"@en, "hat Waschmoglichkeit"@de ;
	rdfs:domain mv:FuelStation ;
	rdfs:range rdfs:Literal .

mv:hasWCFacility
	a rdf:Property, owl:DatatypeProperty ;
	rdfs:comment "Indicate whether Filling Station has WC Facility or not" ;
	rdfs:label "has WC facility"@en, "hat WC Fazilitat"@de ;
	rdfs:domain mv:FuelStation ;
	rdfs:range rdfs:Literal .

mv:hasWheelChairEnabled
	a rdf:Property, owl:DatatypeProperty ;
	rdfs:comment "Indicate whether Filling Station is Wheelchair enabled or not" ;
	rdfs:label "has WC facility"@en, "hat WC Fazilitat"@de ;
	rdfs:domain mv:FuelStation ;
	rdfs:range rdfs:Literal .


mv:offersAccess
	a rdf:Property, owl:DatatypeProperty ;
	rdfs:comment "Indicates for which people access is permitted." ;
	rdfs:label "offers access"@en, "bietet Zugang"@de ;
	rdfs:domain mv:ChargingStation ;
	rdfs:range rdfs:Literal .

mv:offersBooking
	a rdf:Property, owl:DatatypeProperty ;
	rdfs:comment "Indicates whether charging Station offers booking option or not." ;
	rdfs:label "offers booking"@en, "angebote Buchung"@de ;
	rdfs:domain mv:ChargingStation ;
	rdfs:range rdfs:Literal .

mv:offersPlugTypes
	a rdf:Property, owl:DatatypeProperty ;
	rdfs:comment "Indicates which are the offered plug types in the charging Station." ;
	rdfs:label "offers plug type"@en, "bietet Steckertypen"@de ;
	rdfs:domain mv:ChargingStation ;
	rdfs:range rdfs:Literal .

mv:openingHours
	a rdf:Property, owl:DatatypeProperty ;
	rdfs:comment "Indicates the opening hours of the filling station." ;
	rdfs:label "opening hours"@en, "offnungszeiten"@de ;
	rdfs:domain mv:FillingStation ;
	rdfs:range rdfs:Literal .

mv:PaymentMethod
	a rdf:Property, owl:DatatypeProperty ;
	rdfs:comment "Indicates which type of payment is available." ;
	rdfs:label "payment method"@en, "zahlungsmethode"@de ;
	rdfs:domain mv:FillingStation ;
	rdfs:range rdfs:Literal .